skim all cases of progress

proof/iu_system/decl/prop_type_safety.v
@@ -13,12 +13,12 @@ Admitted.
 
 Hint Resolve dwf_typ_lc_dtyp : core.
 
-Fixpoint var_dom (e : denv) : atoms :=
-  match e with 
-  | nil => empty
-  | ((x, dbind_typ T) :: e') => add x (var_dom e')
-  | (_ :: e') => var_dom e'
-  end.
+Inductive empty_var_dom : denv -> Prop :=
+  | evd_empty : empty_var_dom nil
+  | evd_empty_tvar : forall E X, empty_var_dom E -> empty_var_dom ((X , dbind_tvar_empty) :: E)
+  | evd_empty_stvar : forall E SX, empty_var_dom E -> empty_var_dom  ((SX , dbind_stvar_empty) :: E)
+.
+
 
 (* Lemma canonical_form_abs : forall E e m,
   dtyping E e m dtyp_bot -> 
@@ -33,44 +33,71 @@ Proof.
   - inversion H1.
   - inversion H1. *)
 
+Hint Constructors empty_var_dom : core.
+
+Theorem bind_var_var_dom_not_empty : forall E x T,
+  binds x (dbind_typ T) E -> empty_var_dom E -> False.
+Proof.
+  intros. induction E.
+  - inversion H.
+  - destruct a. destruct b.
+    + inversion H.
+      * inversion H1.
+      * inversion H0. auto.
+    + inversion H.
+      * inversion H1.
+      * inversion H0. auto.
+    + inversion H0. 
+Qed.
 
 
-Theorem progress : forall E e m T,
+Theorem progress' : forall E e m T,
   dtyping E e m T ->
-  var_dom E = empty ->
+  empty_var_dom E ->
   is_dvalue_of_dexp e = true \/ exists e', dexp_red e e'.
 Proof.
   intros. dependent induction H; intros; auto.
-  - admit. (* easy : impossible *)
+  - exfalso; eapply bind_var_var_dom_not_empty; eauto.
   - specialize (IHdtyping H1).
     inversion IHdtyping.
     + left. auto.
     + right. destruct H2 as [e']. eauto.
+  (* e1 e2 *)
   - specialize (IHdtyping1 H1). 
     specialize (IHdtyping2 H1). 
     inversion IHdtyping1.
     + inversion IHdtyping2.
       * admit.
-      * destruct H3 as [e2']. right. exists (dexp_app e1 e2'). apply dexpred_app2; auto. rewrite H2. constructor. admit.
+      * destruct H3 as [e2']. right. exists (dexp_app e1 e2'). apply dexpred_app2; auto. rewrite H2. constructor. admit. (* easy : lc *)
     + right. destruct H2 as [e1'].
       exists (dexp_app e1' e2). constructor; auto.
-      admit.
+      admit. (* easy : lc *)
   (* e => BOT *)
   - specialize (IHdtyping H1). inversion IHdtyping.
-    + destruct e; try solve [inversion H2].
-      * inversion H0.
-      * inversion H0.
-      * inversion H0.
-      * inversion H0.
+    + destruct e; try solve [inversion H2; inversion H0].
       * dependent destruction H0. inversion H3.
         right. exists e. constructor.
+        rewrite H5. constructor.
+        admit. admit. (* easy : lc *)
     + right. destruct H2 as [e']. eauto.
-  (* e => ∀ X . T *)
+  (* e @ T *)
   - specialize (IHdtyping H1).
     inversion IHdtyping.
     + admit.
     + right. destruct H2 as [e1']. eauto.
-  (* app *)
+  (* e => ∀ X . T *)
   - inst_cofinites_by L.
     apply H1. simpl. auto.
+Admitted.
+
+
+Theorem progress : forall e m T,
+  dtyping nil e m T ->
+  is_dvalue_of_dexp e = true \/ exists e', dexp_red e e'.
+Proof.
+  intros. eapply progress'; eauto.
 Qed.
+
+
+
+
